specs/ecdsa/Spec.DH.fst
@@ -14,41 +14,28 @@ open Spec.ECC.Curves
 (* Initiator *)
 val ecp256_dh_i: #c: curve 
   -> scalar_bytes #c
-  -> tuple3 (lbytes (getCoordinateLen c)) (lbytes (getCoordinateLen c)) bool
+  -> tuple2 (point #c #Affine) bool
 
 let ecp256_dh_i #c s =
-  let xN, yN, zN = secret_to_public #c s in
-  if isPointAtInfinity #Jacobian (xN, yN, zN) then
-    nat_to_bytes_be (getCoordinateLen c) xN, 
-    nat_to_bytes_be (getCoordinateLen c) yN, 
-    false
+  let p = secret_to_public #c s in 
+  if isPointAtInfinity p then 
+    (fromJacobianCoordinatesTest #c (_norm p), false)
   else
-    nat_to_bytes_be (getCoordinateLen c) xN, 
-    nat_to_bytes_be (getCoordinateLen c) yN, 
-    true
-
+    (fromJacobianCoordinatesTest #c (_norm p), true)
 
 (* Responder *)
 val ecp256_dh_r: #c: curve 
-  -> lbytes (getCoordinateLen c) 
-  -> lbytes (getCoordinateLen c) 
+  -> pubKey: tuple2 nat nat
   -> scalar_bytes #c
-  -> tuple3 (lbytes (getCoordinateLen c)) (lbytes (getCoordinateLen c)) bool
+  -> tuple2 (point #c #Affine) bool
 
-let ecp256_dh_r #c x y s =
-  let x_, y_ = nat_from_bytes_be x, nat_from_bytes_be y in 
-  let pointJacX, pointJacY, pointJacZ = toJacobianCoordinates (x_, y_) in 
-  if verifyQValidCurvePointSpec #c (pointJacX, pointJacY, pointJacZ) then 
-    let xN, yN, zN = scalar_multiplication #c s (pointJacX, pointJacY, pointJacZ) in
-    if isPointAtInfinity #Jacobian (xN, yN, zN) then
-      nat_to_bytes_be (getCoordinateLen c) xN, 
-      nat_to_bytes_be (getCoordinateLen c) yN, 
-      false
-    else
-      nat_to_bytes_be (getCoordinateLen c) xN, 
-      nat_to_bytes_be (getCoordinateLen c) yN, 
-      true
+let ecp256_dh_r #c pubKey scalar  =
+  let pk = toJacobianCoordinates pubKey in 
+  if not (verifyQValidCurvePointSpec #c pk) then
+    (0, 0), false
   else
-      nat_to_bytes_be (getCoordinateLen c) 0, 
-      nat_to_bytes_be (getCoordinateLen c) 0, 
-      false
+    let pk_scalar = scalar_multiplication #c scalar pk in
+    if isPointAtInfinity pk_scalar then 
+      (fromJacobianCoordinatesTest #c (_norm pk_scalar), false)
+    else 
+      (fromJacobianCoordinatesTest #c (_norm pk_scalar), true)
